books/centaur/fgl/gatecount.lisp
@@ -1,0 +1,179 @@
+; FGL - A Symbolic Simulation Framework for ACL2
+; Copyright (C) 2008-2013 Centaur Technology
+;
+; Contact:
+;   Centaur Technology Formal Verification Group
+;   7600-C N. Capital of Texas Highway, Suite 300, Austin, TX 78731, USA.
+;   http://www.centtech.com/
+;
+; License: (An MIT/X11-style license)
+;
+;   Permission is hereby granted, free of charge, to any person obtaining a
+;   copy of this software and associated documentation files (the "Software"),
+;   to deal in the Software without restriction, including without limitation
+;   the rights to use, copy, modify, merge, publish, distribute, sublicense,
+;   and/or sell copies of the Software, and to permit persons to whom the
+;   Software is furnished to do so, subject to the following conditions:
+;
+;   The above copyright notice and this permission notice shall be included in
+;   all copies or substantial portions of the Software.
+;
+;   THE SOFTWARE IS PROVIDED "AS IS", WITHOUT WARRANTY OF ANY KIND, EXPRESS OR
+;   IMPLIED, INCLUDING BUT NOT LIMITED TO THE WARRANTIES OF MERCHANTABILITY,
+;   FITNESS FOR A PARTICULAR PURPOSE AND NONINFRINGEMENT. IN NO EVENT SHALL THE
+;   AUTHORS OR COPYRIGHT HOLDERS BE LIABLE FOR ANY CLAIM, DAMAGES OR OTHER
+;   LIABILITY, WHETHER IN AN ACTION OF CONTRACT, TORT OR OTHERWISE, ARISING
+;   FROM, OUT OF OR IN CONNECTION WITH THE SOFTWARE OR THE USE OR OTHER
+;   DEALINGS IN THE SOFTWARE.
+;
+; Original author: Sol Swords <sswords@centtech.com>
+
+(in-package "FGL")
+
+(include-book "add-primitives")
+(include-book "gatecount-stub")
+(include-book "gatecount-base")
+(local (include-book "std/lists/resize-list" :dir :system))
+(local (include-book "primitive-lemmas"))
+
+(def-formula-checks gatecount-formula-checks
+  (gatecount support-vars))
+
+(define fgl-object-gatecount ((x fgl-object-p) interp-st)
+  :guard (and (bfr-mode-is :aignet (interp-st-bfr-mode))
+              (interp-st-bfr-listp (fgl-object-bfrlist x)))
+  :returns (count natp :rule-classes :type-prescription)
+  (with-local-stobj bitarr
+    (mv-let (count bitarr)
+      (stobj-let ((logicman (interp-st->logicman interp-st)))
+                 (bitarr)
+                 (b* ((bitarr (resize-bits (+ 1 (bfrstate->bound (logicman->bfrstate))) bitarr))
+                      ((mv bitarr seen) (fgl-object-mark-gates x bitarr logicman nil)))
+                   (fast-alist-free seen)
+                   bitarr)
+                 (b* ((count (bitarr-count bitarr)))
+                   (mv count bitarr)))
+      count)))
+               
+(define aignet-collect-marked-bvars ((n natp)
+                                     bitarr
+                                     bvar-db
+                                     aignet)
+  :returns (var-list)
+  :guard (and (<= (base-bvar bvar-db) n)
+              (<= n (aignet::num-ins aignet))
+              (eql (next-bvar bvar-db) (aignet::num-ins aignet))
+              (<= (aignet::num-fanins aignet) (bits-length bitarr)))
+  :measure (nfix (- (aignet::num-ins aignet) (nfix n)))
+  (b* (((when (mbe :logic (zp (- (aignet::num-ins aignet) (nfix n)))
+                   :exec (eql (aignet::num-ins aignet) n)))
+        nil)
+       (id (aignet::innum->id n aignet))
+       ((when (eql 0 (get-bit id bitarr)))
+        (aignet-collect-marked-bvars (1+ (lnfix n)) bitarr bvar-db aignet))
+       (var (get-bvar->term n bvar-db)))
+    (cons var
+          (aignet-collect-marked-bvars (1+ (lnfix n)) bitarr bvar-db aignet))))
+
+(define fgl-object-support-vars ((x fgl-object-p) interp-st)
+  :guard (and (bfr-mode-is :aignet (interp-st-bfr-mode))
+              (interp-st-bfr-listp (fgl-object-bfrlist x))
+              (interp-st-bfrs-ok interp-st))
+  :returns (vars)
+  :guard-hints (("goal" :in-theory (enable interp-st-bfrs-ok bfr-nvars)))
+  (with-local-stobj bitarr
+    (mv-let (vars bitarr)
+      (stobj-let ((logicman (interp-st->logicman interp-st))
+                  (bvar-db  (interp-st->bvar-db interp-st)))
+                 (vars bitarr)
+                 (b* ((bitarr (resize-bits (+ 1 (bfrstate->bound (logicman->bfrstate))) bitarr))
+                      ((mv bitarr seen) (fgl-object-mark-gates x bitarr logicman nil)))
+                   (fast-alist-free seen)
+                   (stobj-let ((aignet (logicman->aignet logicman)))
+                              (vars)
+                              (aignet-collect-marked-bvars (base-bvar bvar-db)
+                                                           bitarr bvar-db aignet)
+                              (mv vars bitarr)))
+                 (mv vars bitarr))
+      vars)))
+                       
+                 
+(local (defthm fgl-ev-context-equv-forall-extensions-trivial
+         (implies (acl2::rewriting-negative-literal
+                   `(fgl-ev-context-equiv-forall-extensions ,contexts ,obj ,term ,eval-alist))
+                  (iff (fgl-ev-context-equiv-forall-extensions contexts obj term eval-alist)
+                       (and 
+                        (equal (fgl-ev-context-fix contexts (fgl-ev term eval-alist))
+                               (fgl-ev-context-fix contexts obj))
+                        (hide (fgl-ev-context-equiv-forall-extensions contexts obj term eval-alist)))))
+         :hints (("goal" :expand ((:free (x) (hide x)))
+                  :use ((:instance fgl-ev-context-equiv-forall-extensions-necc
+                         (ext eval-alist)))
+                  :in-theory (disable fgl-ev-context-equiv-forall-extensions-necc)))))
+
+(local (in-theory (disable fgl-ev-context-equiv-forall-extensions)))
+
+
+(def-fgl-binder-meta gatecount-binder
+  (b* (((unless (bfr-mode-is :aignet (interp-st-bfr-mode)))
+        (cw "Failed to compute gatecount -- not in aignet mode~%")
+        (mv nil nil nil nil interp-st state))
+       (count (fgl-object-gatecount arg interp-st)))
+    (mv t (kwote count) nil nil interp-st state))
+  :formula-check gatecount-formula-checks
+  :prepwork ((local (in-theory (enable gatecount))))
+  :origfn gatecount :formals (arg))
+
+(def-fgl-binder-meta support-vars-binder
+  (b* (((unless (bfr-mode-is :aignet (interp-st-bfr-mode)))
+        (cw "Failed to compute gatecount -- not in aignet mode~%")
+        (mv nil nil nil nil interp-st state))
+       (vars (fgl-object-support-vars arg interp-st)))
+    (mv t (kwote vars) nil nil interp-st state))
+  :formula-check gatecount-formula-checks
+  :prepwork ((local (in-theory (enable support-vars))))
+  :origfn support-vars :formals (arg))
+
+
+
+(def-fgl-program gatecount! (x)
+  (gatecount no-var x))
+
+
+(defmacro fgl-gatecount (name expr)
+  `(let ((,name ,expr))
+     (fgl-prog2 (cw "~x0 gatecount: ~x1~%" ',name (gatecount! ,name))
+                     ,name)))
+
+(defxdoc fgl-gatecount
+  :parents (fgl-debugging)
+  :short "Display how many AIG gates are used in the symbolic representation of an object"
+  :long "<p>Logically, this returns its second argument; its first argument
+should be a variable symbol.  This counts the number of AIG gates that are used
+in the symbolic representation of the object (second argument) and prints that
+out as a debugging message.</p>
+
+<p>If you want to do anything else with the gatecount, you can get that count
+using @('(gatecount! x)') under an @(see unequiv) context, or using the binder
+form @('(gatecount free-var x)') in a rewrite rule.</p>")
+
+(def-fgl-program support-vars! (x)
+  (support-vars no-var x))
+
+
+(defmacro fgl-support-vars (name expr)
+  `(let ((,name ,expr))
+     (fgl-prog2 (cw "~x0 support-vars: ~x1~%" ',name (support-vars! ,name))
+                ,name)))
+
+(defxdoc fgl-support-vars
+  :parents (fgl-debugging)
+  :short "Display the list of objects corresponding to the Boolean variables used in the symbolic representation of an object"
+  :long "<p>Logically, this returns its second argument; its first argument
+should be a variable symbol.  This finds which Boolean variables are used in
+the representation of the object (second argument) and prints out the objects
+from which those variables were generated.</p>
+
+<p>If you want to do anything else with this list of objects, you can get that
+list using @('(support-vars! x)') under an @(see unequiv) context, or using the binder
+form @('(support-vars free-var x)') in a rewrite rule.</p>")
